\documentclass[answers,11pt]{exam}
% \usepackage{pslatex}
\usepackage{xparse}
\usepackage{graphicx}
\DeclareGraphicsExtensions{.jpg, .png}
\usepackage{amsmath}
\usepackage{fourier}
%\usepackage{amsfonts}
\usepackage{enumerate}
\usepackage{siunitx}
\firstpageheader{}{}{}
\runningheader{\textbf{Spring 2013}}
 {}
 {\textbf{Math 352}}
 %{\emph{Page \thepage~of \numpages}}
\runningheadrule
\setlength{\parskip}{1ex}
\setlength{\parindent}{0pt}
\pagestyle{head}
%\newcommand{\N}{\mathbb{N}}
%\newcommand{\Z}{\mathbb{Z}}
%\newcommand{\R}{\mathbb{R}}
%\newcommand{\dwrspace}[1]{\vspace*{\stretch{#1}}}
\NewDocumentCommand\N{}{\mathbf{N}}
\NewDocumentCommand\R{}{\mathbf{R}}
\NewDocumentCommand\Z{}{\mathbf{Z}}
\NewDocumentCommand\Q{}{\mathbf{Q}}
\NewDocumentCommand\dwrspace{m}{\vspace*{\stretch{#1}}}
\begin{document}
\noindent
\textbf{{\large Mathematics 352 \\ Undetermined Coefficients}}
% \hfill Name: \underline{\hspace{0.5in}Answers\hspace{2in}}

\noindent
April 5, 2013 \hfill Name: \underline{\hspace{3in}} 

\noindent
Due: April 10, 2013

\noindent
\begin{figure}[h]
\centering
\begin{minipage}[b]{0.85\linewidth}
\textbf{Introduction.} In this activity you will get some practice using the method of undetermined coefficients to solve inhomogeneous differential equations $ay'' + by' + cy = g(t)$ in which the inhomogeneous term $g(t)$ is a combination of polynomial, exponential, or trigonometric functions.
\end{minipage}
\end{figure}

Recall that the general solution to the inhomogeneous differential equation $ay'' + by' + cy = g(t)$ is $y_c + Y$, where the \emph{complementary solution} $y_c = c_1 y_1 + c_2 y_2$ is the general solution of the \emph{associated homogeneous equation} and $Y$ is \emph{any} particular solution of the inhomogeneous equation.

\begin{questions}

\question Find the \emph{complementary solution} of $y'' - 4y' - 12y = 3e^{5t}$. This is always the first step. You should always do this \emph{before} attempting to find a particular solution $Y$.

\begin{solution}
	The complementary solution is given by the roots of the characteristic equation for the associated homogeneous system, $r^2 - 4r - 12 = 0$. The left-hand side factors as $(r-6)(r+2)$, so a fundamental set of solutions is $y_1 = e^{6t}$ and $y_2 = e^{-2t}$, and therefore the complementary solution is
    \[
        y_c = c_1 e^{6t} + c_2 e^{-2t}.
    \]
\end{solution}

\question Use the method of undetermined coefficients to find a particular solution $Y$ of $y'' - 4y' - 12y = 3e^{5t}$.

\begin{solution}
	Since $e^{5t}$ does \emph{not} appear in the complementary solution, we look for a solution of the form $Ae^{5t}$. Letting $Y$ equal this last expression and differentiating, we find $Y' = 5Y$ and $Y'' = 25Y$. Therefore, on substitution of $Y$ into the left-hand side of the differential equation, we obtain $25Y - 4(5Y) - 12Y = -7Y$. Therefore we must have $-7A = 3$, whence $A = -3/7$. The particular solution so obtained is
    \[
        Y = -3/7 e^{5t}.
    \]
\end{solution}

\question Check, by direct substitution, that your function $Y$ really is a particular solution.

\begin{solution}
	We have $Y' = -15/7 e^{5t}$ and $Y'' = -75/7 e^{5t}$. We compute:
    \begin{align*}
        Y'' - 4Y' - 12Y &= (-75/7 - 4(-15/7) - 12(-3/7)) e^{5t} \\
        &= (-75/7 + 60/7 + 36/7) e^{5t} \\
        &= (21/7) e^{5t} \\
        &= 3e^{5t},
    \end{align*}
    as required.
\end{solution}

\question No further calculation is necessary to write down the general solution of the inhomogeneous equation: do so below.

\begin{solution}
    The general solution is equal to the complementary solution $y_c$ plus the particular solution $Y$, namely
    \[
      c_1 e^{6t} + c_2 e^{-2t} - \frac{3}{7} e^{5t}.
    \]
\end{solution}

\question Use the method of undetermined coefficients to find a particular solution $Y$ of $y'' - 4y' - 12y = \sin{(2t)}$. 

\begin{solution}
	Here the method calls for a particular solution of the form $Y = A \cos{(2t)} + B \sin{(2t)}$. Differentiating, we find
    \begin{align*}
        Y' &= 2B \cos{(2t)} - 2A \sin{(2t)} \\
        Y'' &= -4A \cos{(2t)} - 4B \sin{(2t)}.
    \end{align*}
    Substituting, we observe now that
    \begin{align*}
        Y'' - 4Y' - 12Y &= (-4A - 4(2B) - 12A) \cos{(2t)} + (-4B - 4(-2A) - 12B) \sin{(2t)} \\
        &= (-16A - 8B) \cos{(2t)} + (8A - 16B) \sin{(2t)}.
    \end{align*}
    Equating like coefficients, we obtain a $2 \times 2$ system of linear equations
    \begin{align*}  
        -16 A - 8 B &= 0 \\
        8A - 16B &= 1.
    \end{align*}
    The first equation entails that $B = -2A$. Substitution into the second yields $8A - 16(-2A) = 1$, whence $A = 1/40$. Hence $B = -1/20$ and the particular solution we are seeking is
    \[
        \frac{1}{40} \cos{(2t)} - \frac{1}{20} \sin{(2t)}.
    \]
\end{solution}

\question Verify, by direct substitution, that $Y$ really is a particular solution.

\begin{solution}
	Left to the reader.
\end{solution}

\question Use the method of undetermined coefficients to find a particular solution $Y$ of $y'' - 4y' - 12y = 2t^3 - t + 3$.

\begin{solution}
	Here, the particular solution takes the form $Y = At^3 + Bt^2 + Ct + D$. The derivatives are
    \begin{align*}
        Y' &= 3At^2 + 2Bt + C \\
        Y'' &= 6At + 2B.
    \end{align*}    
    Substitution yields 
    \begin{align*}
        Y'' - 4Y' - 12Y &= (6At + 2B) - 4(3At^2 + 2Bt + C) - 12(At^3 + Bt^2 + Ct + D)\\
        &= -12At^3 + (-12A - 12B)t^2 + (6A - 8B - 12C)t + (2B - 4C - 12D).
    \end{align*}
    Equating the coefficients of the various monomials then gives the system of linear equations
    \begin{align*}
        -12A &= 2 \\
        -12A - 12B &= 0 \\
        6A - 8B - 12C &= -1 \\
        2B - 4C - 12D &= 3.
    \end{align*}
    This is tedious, but there's no helping it. Evidently, $A = -1/6$ and $B = 1/6$. The third equation then becomes $-1 - 4/3 - 12C = -1$, whence $C = -1/9$. Finally, the last equation is $1/3 + 4/9 - 12D = 3$, so that $-12D = 3 - 7/9 = 20/9$ and $D = -5/27$. The desired particular solution is
    \[
        -\frac{1}{6}t^3 + \frac{1}{6}t^2 - \frac{1}{9}t - \frac{5}{27}.
    \]
\end{solution}

\question Verify, by direct substitution, that $Y$ really is a particular solution.

\begin{solution}
    Left, joyfully, to the reader, as are the rest.
\end{solution}

\question Write down the form (including the undetermined coefficients) of initial guesses for the particular solutions if $g(t)$ is the indicated function.

\begin{parts}
    \part $g(t) = 16 e^{7t} \sin{(10t)}$
    \part $g(t) = (9t^2 - 103t) \cos{(t)}$
    \part $g(t) = -e^{-2t} (3 - 5t) \cos{(9t)}$
\end{parts}

\question Solve the initial value problem 
\[
    y'' - 4y' - 12y = 3e^{5t}, \quad y(0) = 18/7,\, y'(0) = -1/7
\]
\end{questions}

\end{document}