\documentclass[answers,11pt]{exam}
% \usepackage{pslatex}
\usepackage{xparse}
\usepackage{graphicx}
\DeclareGraphicsExtensions{.jpg, .png}
\usepackage{amsmath}
\usepackage{fourier}
%\usepackage{amsfonts}
\usepackage{enumerate}
\usepackage{siunitx}
\firstpageheader{}{}{}
\runningheader{\textbf{Spring 2013}}
 {}
 {\textbf{Math 352}}
 %{\emph{Page \thepage~of \numpages}}
\runningheadrule
\setlength{\parskip}{1ex}
\setlength{\parindent}{0pt}
\pagestyle{head}
%\newcommand{\N}{\mathbb{N}}
%\newcommand{\Z}{\mathbb{Z}}
%\newcommand{\R}{\mathbb{R}}
%\newcommand{\dwrspace}[1]{\vspace*{\stretch{#1}}}
\NewDocumentCommand\N{}{\mathbf{N}}
\NewDocumentCommand\R{}{\mathbf{R}}
\NewDocumentCommand\Z{}{\mathbf{Z}}
\NewDocumentCommand\Q{}{\mathbf{Q}}
\NewDocumentCommand\dwrspace{m}{\vspace*{\stretch{#1}}}
\extrawidth{1.0in}
\extraheadheight{-0.5in}
\extrafootheight{-0.5in}
\begin{document}
\noindent
\textbf{{\large Mathematics 352 \\ Variation of Parameters}}
% \hfill Name: \underline{\hspace{0.5in}Answers\hspace{2in}}

\begin{questions}

\question Use variation of parameters to find the general solution of the equation
\[
    y'' - y' - 2y = e^{3t}.
\]

\begin{solution}
    The characteristic polynomial is $(r - 2)(r + 1)$, so $y_1 = e^{2t}$ and $y_2 = e^{-t}$ are a fundamental set of solutions to the associated homogeneous equation. We compute $W(y_1, y_2) = (e^{2t})(-e^{-t}) - (2e^{2t})(e^{-t}) = -3e^{t}$. The variation of parameters formulas yield
    \begin{align*}
        u_1 &= -\int \frac{e^{-t} e^{3t}}{-3e^t} \; dt = \int \frac{e^t}{3} \; dt = \frac{e^t}{3}, \\
        u_2 &= \int \frac{e^{2t} e^{3t}}{-3e^t} \; dt = -\frac{1}{3} \int e^{4t} \; dt = -\frac{1}{12} e^{4t}.
    \end{align*}
    Therefore a particular solution is
    \[
        u_1 y_1 + u_2 y_2 = \frac{1}{3} e^{3t} - \frac{1}{12} e^{3t} = \frac{1}{4} e^{3t}.
    \]
\end{solution}

\question Use variation of parameters to find the general solution of the equation
\[
    y'' - 4y' + 5y = e^{-4x}.
\]

\question Verify that $y_1 = t^2$ and $y_2 = t^{-1}$ are solutions of the equation
\[
    t^2 y'' - 2y = 0.
\]

\question Use variation of parameters to find the general solution of the equation
\[
    t^2 y'' - 2y = 3t^2 - 1.
\]
You can assume $t > 0$ wherever necessary.

\begin{solution}
    As above we let $y_1 = t^2$ and $y_2 = t^{-1}$. Since their Wronskian is 
    \[
        t^2 (-t^{-2}) - 2t(t^{-1}) = -1 -2 = -3,
    \]
    they are an independent set of solutions to the associated homogeneous equation. The variation of parameters equations give
    \begin{align*}
        u_1 &= -\int \frac{t^{-1} (3t^2 - 1)}{-3} \; dt = \frac{1}{3} \int 3t - t^{-1} \; dt = \frac{1}{3} \left(\frac{3}{2} t^2 - \ln |t|\right) = \frac{1}{2} t^2 - \frac{1}{3} \ln |t|, \\
        u_2 &= \int \frac{t^2(3t^2-1)}{-3} \; dt = \frac{1}{3} \int 3t^4 - t^2 \; dt = \frac{1}{3} \left( \frac{3}{5}t^5 - \frac{1}{3}t^3 \right) = \frac{1}{5} t^5 - \frac{1}{9} t^3.
    \end{align*}
\end{solution}

\end{questions}

\end{document}